SimplePCFa: do Progress
Ignore-this: fc6e6b66b6db689a2222122ee4773c09

darcs-hash:20130131121154-08f32-0076696bc3c393f45c34c13ed89930c5254ffd02

devel/Iron/Language/SimplePCFa/Step/Frame.v
@@ -5,8 +5,8 @@ Require Import Iron.Language.SimplePCFa.Value.
 
 (* Frame stacks *)
 (* Holds the continuation while a 'let' expression reduces the bound term. *)
-Inductive frame : Set :=
- | F : forall (t : ty) (x : exp), frame.
+Inductive frame : Type :=
+ | F : ty -> exp -> frame.
 Hint Constructors frame.
 
 Definition stack := list frame.
@@ -15,6 +15,11 @@ Hint Unfold stack.
 
 (* Single step reduction under a frame stack. *)
 Inductive STEPF : stack -> exp -> stack -> exp -> Prop :=
+ | SfStep
+   :  forall fs x1 x2
+   ,  STEPP    x1    x2
+   -> STEPF fs x1 fs x2
+
  | SfPush
    :  forall fs t x1 x2
    ,  STEPF fs             (XLet t x1 x2)
@@ -22,14 +27,10 @@ Inductive STEPF : stack -> exp -> stack -> exp -> Prop :=
 
  | SfPop
    :  forall fs x t v
-   ,  STEPF (fs :> F t x) (XVal v)
-            fs            (substVX 0 v x)
-
- | SfStep
-   :  forall fs x1 x2
-   ,  STEPP x1 x2
-   -> STEPF fs x1 fs x2.
+   ,  STEPF (fs :> F t x)  (XVal v)
+            fs             (substVX 0 v x).
 Hint Constructors STEPF.
+
 
 
 (** Multi-step evaluation under a frame stack *)
@@ -56,5 +57,4 @@ Inductive STEPRS : stack -> exp -> stack -> exp -> Prop :=
    ,  STEPRS fs1 x1 fs2 x2 -> STEPF fs2 x2 fs3 x3 
    -> STEPRS fs1 x1 fs3 x3.
 Hint Constructors STEPRS.
-
 
