devel/Iron/Language/SimplePCFa/Step.v
@@ -2,4 +2,5 @@
 Require Export Iron.Language.SimplePCFa.Step.Frame.
 Require Export Iron.Language.SimplePCFa.Step.Prim.
 Require Export Iron.Language.SimplePCFa.Step.Term.
+Require Export Iron.Language.SimplePCFa.Step.TfJudge.
 
