devel/Iron/Language/SimplePCFa/Step/Progress.v
@@ -1,0 +1,90 @@
+
+Require Import Iron.Language.SimplePCFa.Step.Frame.
+Require Import Iron.Language.SimplePCFa.Step.TfJudge.
+Require Import Iron.Language.SimplePCFa.Value.
+
+
+Definition done (fs : stack) (x : exp)
+ := fs = nil /\ (exists v, x = XVal v).
+Hint Unfold done.
+
+Lemma progress
+ :  forall fs x t
+ ,  TYPEC nil fs x t
+ -> done fs x \/ (exists fs' x', STEPF fs x fs' x').
+Proof.
+ intros fs x t HC.
+ gen fs t.
+ induction x; intros.
+
+ Case "XVal".
+  induction fs.
+   left.
+    unfold done. rip.
+    exists v. auto.
+   right.
+    destruct a as [t3 x3].
+    exists fs.
+    exists (substVX 0 v x3).
+    eauto.
+
+ Case "XLet".
+  right.
+  exists (fs :> F t x2).
+  exists x1. 
+  auto.
+
+ Case "XApp".
+  right.
+  exists fs.
+  inverts HC.
+  destruct v; nope.
+   SCase "v1 = VLam".
+    exists (substVX 0 v0 e).
+    eauto.
+   SCase "v1 = VFix".
+    exists (XApp (substVV 0 (VFix t0 v) v) v0).
+    eauto.
+
+ Case "XOp1".
+  right.
+  exists fs.
+   destruct o.
+
+   SCase "OSucc".
+    destruct v; nope.
+    SSCase "VConst". 
+     destruct c; nope.
+     exists (XVal (VConst (CNat (S n)))).
+      auto.
+    SSCase "VFix".
+     admit. (* wrong: fixpoints aren't values. *)
+
+   SCase "OPred".
+    destruct v; nope.
+    SSCase "VConst".
+     destruct c; nope.
+     destruct n; eauto.
+    SSCase "VFix".
+     admit. (* wrong: fixpoints aren't values *)
+     
+  SCase "OIsZero".
+   destruct v; nope.
+   SSCase "VConst".
+    destruct c; nope.
+    destruct n; eauto.
+   SSCase "VFix".
+    admit. (* wrong: fixpoints aren't values *)
+    
+ Case "XIf".
+  right.
+  exists fs.
+  destruct v; nope.
+  SSCase "VConst".
+   destruct c; nope.
+   destruct b; eauto.
+  SSCase "VFix".
+   admit.   (* wrong: fixpoints aren't values. *)
+Qed.
+
+
