devel/Iron/Language/SimplePCFa/Step/TfJudge.v
@@ -1,0 +1,29 @@
+
+Require Import Iron.Language.SimplePCFa.Step.Frame.
+Require Import Iron.Language.SimplePCFa.Step.Prim.
+Require Import Iron.Language.SimplePCFa.Value.
+
+
+(* Type of a frame stack.
+   The frame stack is like a continuation that takes an expression of a certain
+   type and produces a new expression. *)
+Inductive TYPEF : tyenv -> stack -> ty -> ty -> Prop := 
+ | TfNil 
+   :  forall te t
+   ,  TYPEF  te nil t t
+
+ | TfCons
+   :  forall te fs t1 t2 t3 x2
+   ,  TYPEX (te :> t1) x2 t2
+   -> TYPEF  te fs t2 t3
+   -> TYPEF  te (fs :> F t1 x2) t1 t3.
+
+
+(* Type of an expression in a frame context. *)
+Inductive TYPEC : tyenv -> stack -> exp -> ty -> Prop :=
+ | TcExp
+   :  forall te fs x t1 t2
+   ,  TYPEF te fs t1 t2
+   -> TYPEX te x  t1
+   -> TYPEC te fs x t2.
+
